1) designed an aa database    a) we added a modified analysis pass MyAliasAnalysisEvaluation.cpp that was       extended from the AliasAnalysisEvaluation.cpp, but makes the output       compact and simple to reduce size.
      The aa result is from -basicaa that is the default one used by LLVM GVN.

      We only store the no-alias and must-alias queries, the rest ones are may-
      alias for sure. In practice, on average, each function may take 200
      pointers, so we have 100 * 199 pairs of queries. Among them, 50% is may-
      alias, 10% is no-alias, 40% is must-alias. The entire size of the DB is
      300K - 10M.

      Data for each function are stored in the order of the functions.

      The generation of DB takes 1s - 2m. But most of the time (95%) is for the
      C ++ STL err output (flushed frequently), which can be optimized later.

      The following aa information is not stored in DB yet.
      A) constant pointers (globals, or cast/gep that depend on globals)
      B) callsite effects

    b) In OCaml, we traverse the DB in the program order as they are stored,
      and only store aa queries for the compiling function in a hashtable. We
      never need to randomly access the DB.

      So far, 0.1% of time (by Cachegrind) is for the DB access in our
      compilation. So, it is not an issue. We can replace the hashtable by a
      trie if needed.

2) The real performance bottleneck is from the ad-hoc mem-dependency computation.
   It was replaced by a fast fixpoint based on available expression computation.
   0.99go is working after the fix.

   To make the analyis incremental, we can store the bitvector result at fixpoint
   for each pair of query. Then when program is updated, the new analysis can be
   initalized from the cached result, but not from the standard initial value.
   This may make the analysis converged faster. But so far, we have not done this.

NOTE: OcaIDE does not support ml files with capitalized names when debugging.
This was why in our Vellvm development all Coq files are named by small letters...




git-svn-id: https://webdav.seas.upenn.edu/svn/sol/vol@3393 eef5ea85-cc2e-0410-bd84-0fae1f012da8

src/Transforms/gvn.v
@@ -263,31 +263,50 @@ match c with
 | _ => None
 end.
 
-Definition is_aliasing (pv1:value) (t1:typ) (pv2:value) (t2:typ) : bool := true.
+Parameter is_no_alias_id: id -> id -> bool.
+
+Definition is_no_alias (pv1:value) (t1:typ) (pv2:value) (t2:typ) : bool := 
+match pv1, pv2 with
+| value_id id1, value_id id2 => is_no_alias_id id1 id2
+| value_const (const_gid _ id1), value_const (const_gid _ id2) => 
+    negb (id_dec id1 id2)
+| _, _ => false
+end.
 
 Definition kill_aliased_loadstores (inscope: lcmds) (pv1:value) (t1:typ) 
  : lcmds :=
  List.filter (fun data => 
               match data with
-              | (_, insn_load _ t2 pv2 _) => negb (is_aliasing pv1 t1 pv2 t2)
-              | (_, insn_store _ t2 _ pv2 _) => negb (is_aliasing pv1 t1 pv2 t2)
+              | (_, insn_load _ t2 pv2 _) => is_no_alias pv1 t1 pv2 t2
+              | (_, insn_store _ t2 _ pv2 _) => is_no_alias pv1 t1 pv2 t2
               | (_, _) => true
               end) inscope.
 
-Fixpoint lookup_redundant_load (inscope: lcmds) t1 pv1 al1 
+Parameter is_must_alias_id: id -> id -> bool.
+
+Definition is_must_alias (pv1:value) (t1:typ) (pv2:value) (t2:typ) : bool :=
+match pv1, pv2 with
+| value_id id1, value_id id2 => 
+    if id_dec id1 id2 then true else is_must_alias_id id1 id2
+| value_const (const_gid _ id1), value_const (const_gid _ id2) => id_dec id1 id2
+| _, _ => false
+end. 
+
+Fixpoint lookup_redundant_load (inscope: lcmds) t1 pv1
   : option (l * id * value) :=
 match inscope with
 | nil => None
 | (l0,c)::inscope' =>
-    if (rhs_dec (rhs_load t1 pv1 al1) (rhs_of_cmd c)) 
-    then Some (l0, getCmdLoc c, value_id (getCmdLoc c))
-    else 
-      match c with
-      | insn_store id0 t1' v0' pv1' _ => 
-          if (t1 =t= t1') && valueEqB pv1 pv1' then Some (l0, id0, v0')
-          else lookup_redundant_load inscope' t1 pv1 al1
-      | _ => lookup_redundant_load inscope' t1 pv1 al1
-      end
+    match c with
+    | insn_load _ t1' pv1' _ =>
+       if (is_must_alias pv1' t1' pv1 t1 && (t1 =t= t1')) then
+         Some (l0, getCmdLoc c, value_id (getCmdLoc c))
+       else lookup_redundant_load inscope' t1 pv1
+    | insn_store id0 t1' v0' pv1' _ => 
+       if (is_must_alias pv1' t1' pv1 t1 && (t1 =t= t1')) then Some (l0, id0, v0')
+       else lookup_redundant_load inscope' t1 pv1
+    | _ => lookup_redundant_load inscope' t1 pv1
+    end
 end.
 
 Definition block_doesnt_kill (b: block) (pv1:value) (t1:typ) : bool :=
@@ -296,7 +315,7 @@ List.fold_left
   (fun (acc:bool) c =>
    if acc then
      match (mem_effect c) with
-     | Some (pv2, t2) => negb (is_aliasing pv1 t1 pv2 t2)
+     | Some (pv2, t2) => is_no_alias pv1 t1 pv2 t2
      | None => 
          match c with
          | insn_call _ _ _ _ _ _ => false
@@ -319,10 +338,101 @@ List.fold_left
   (fun (acc:bool) c =>
    if acc then
      match (mem_effect c) with
-     | Some (pv2, t2) => negb (is_aliasing pv1 t1 pv2 t2)
+     | Some (pv2, t2) => is_no_alias pv1 t1 pv2 t2
      | None => true
      end
    else acc) (split_cmds cs id1) true.
+
+Module LBooleanInv <: SEMILATTICE_WITH_TOP.
+
+Definition t := bool.
+
+Definition eq (x y: t) := (x = y).
+Definition eq_refl: forall x, eq x x := (@refl_equal t).
+Definition eq_sym: forall x y, eq x y -> eq y x := (@sym_equal t).
+Definition eq_trans: forall x y z, eq x y -> eq y z -> eq x z := (@trans_equal t).
+
+Definition beq : t -> t -> bool := eqb.
+
+Lemma beq_correct: forall x y, beq x y = true -> eq x y.
+Proof eqb_prop.
+
+Definition ge (x y: t) : Prop := x = false \/ y = true \/ x = y.
+
+Lemma ge_refl: forall x y, eq x y -> ge x y.
+Proof. unfold ge; tauto. Qed.
+
+Lemma ge_trans: forall x y z, ge x y -> ge y z -> ge x z.
+Proof. unfold ge; intuition congruence. Qed.
+
+Lemma ge_compat: forall x x' y y', eq x x' -> eq y y' -> ge x y -> ge x' y'.
+Proof.
+  unfold eq; intros; congruence.
+Qed.
+
+Definition bot := true.
+
+Lemma ge_bot: forall x, ge x bot.
+Proof. destruct x; compute; tauto. Qed.
+
+Definition top := false.
+
+Lemma ge_top: forall x, ge top x.
+Proof. unfold ge, top; tauto. Qed.
+
+Definition lub (x y: t) := x && y.
+
+Lemma lub_commut: forall x y, eq (lub x y) (lub y x).
+Proof. intros; unfold eq, lub. apply andb_comm. Qed.
+
+Lemma ge_lub_left: forall x y, ge (lub x y) x.
+Proof. destruct x; destruct y; compute; tauto. Qed.
+
+End LBooleanInv.
+
+Module AvailableDS := Dataflow_Solver(LBooleanInv)(AtomNodeSet).
+
+Definition available_transf (f:fdef) (src tgt:l) (id1:id) (pv1:value) (t1:typ) 
+  (curr:l) (input:bool) : bool :=
+if l_dec curr src then true
+else
+  if l_dec curr tgt then
+    match lookupBlockViaLabelFromFdef f curr with
+    | None => false
+    | Some b => cmds_doesnt_kill b id1 pv1 t1 && input
+    end
+  else 
+    match lookupBlockViaLabelFromFdef f curr with
+    | None => false
+    | Some b => block_doesnt_kill b pv1 t1 && input
+    end
+.
+
+Fixpoint available_init_aux (bs : blocks) (src:l) 
+  (acc: list (l * bool)) : list (l * bool) :=
+match bs with
+| nil => acc
+| block_intro l0 _ _ _ :: bs' => 
+    available_init_aux bs' src
+      ((l0, if (l_dec l0 src) then true else false) :: acc)
+end.
+
+Definition available_init (f:fdef) src : list (l * bool) :=
+match f with
+| fdef_intro _ bs => available_init_aux bs src nil
+end.
+
+Definition available_aux (f:fdef) (src tgt:l) (id1:id) (pv1:value) (t1:typ) 
+  : option (AMap.t bool) :=
+AvailableDS.fixpoint (successors f) (available_transf f src tgt id1 pv1 t1) 
+  ((src, LBooleanInv.bot) :: nil).
+
+Definition fdef_doesnt_kill (f:fdef) (src tgt:l) (id1:id) (pv1:value) 
+  (t1:typ) : bool :=
+match available_aux f src tgt id1 pv1 t1 with  
+| None => false
+| Some rs => AMap.get tgt rs
+end.
 
 Program Fixpoint fdef_doesnt_kill_aux (f:fdef) (preds : ATree.t ls) 
   (nvisited:list l) (src curr target:l) (id1:id) (pv1:value) (t1:typ)
@@ -356,12 +466,12 @@ end.
 Next Obligation. 
   apply remove_in_length; auto.
 Qed.
-
+(*
 Definition fdef_doesnt_kill (f:fdef) (src target:l) (id1:id) (pv1:value) 
   (t1:typ) : bool :=
 fdef_doesnt_kill_aux f (make_predecessors (successors f)) (bound_fdef f)
   src target target id1 pv1 t1.
-
+*)
 Definition kill_loadstores (inscope: lcmds) : lcmds :=
  List.filter (fun data => 
               match data with
@@ -393,7 +503,7 @@ else
   match c with 
   | insn_load id1 t1 pv1 al1 =>
     if does_load_elim tt then
-      match lookup_redundant_load inscope t1 pv1 al1 with
+      match lookup_redundant_load inscope t1 pv1 with
       | None => (f, changed, (l1,c)::inscope)
       | Some (l0, id0, v0) => 
           if fdef_doesnt_kill f l0 l1 id1 pv1 t1 then
@@ -679,6 +789,8 @@ Definition dce_fdef (f:fdef) : fdef :=
 let '(fdef_intro fh bs) := f in
 fold_left (fun f1 b => dce_block f1 b) bs f.
 
+Parameter read_aa_from_fun: id -> bool.
+
 Definition opt_fdef (f:fdef) : fdef :=
 match getEntryBlock f, reachablity_analysis f with
 | Some (block_intro root _ _ _), Some rd =>
@@ -692,7 +804,7 @@ match getEntryBlock f, reachablity_analysis f with
         create_dtree_from_chain acc chain) 
       chains (DT_node root DT_nil) in
     if print_reachablity rd && print_dominators b dts && 
-       print_dtree dt then
+       print_dtree dt && read_aa_from_fun (getFdefID f) then
        match fix_temporary_fdef 
                (SafePrimIter.iterate _ (opt_step dt dts rd) 
                  (dce_fdef f)) with
@@ -744,14 +856,18 @@ Next Obligation.
 Qed.
 *)
 
+Parameter open_aa_db : unit -> bool.
+
 Definition opt (m:module) : module :=
 let '(module_intro los nts ps) := m in
-module_intro los nts 
-  (List.rev (fold_left (fun acc p =>
-                        match p with
-                        | product_fdef f => product_fdef (opt_fdef f)
-                        | _ => p
-                        end::acc) ps nil)).
+if open_aa_db tt then
+  module_intro los nts 
+    (List.rev (fold_left (fun acc p =>
+                          match p with
+                          | product_fdef f => product_fdef (opt_fdef f)
+                          | _ => p
+                          end::acc) ps nil))
+else m.
 
 (*****************************)
 (*
